Foundation/Modal/Boxdot/Grz_S.lean
@@ -3,10 +3,8 @@ import Foundation.Modal.Boxdot.GL_S
 
 namespace LO.Modal.Logic
 
-lemma iff_provable_Grz_provable_boxdot_S {φ : Formula _} : φᵇ ∈ Logic.S ↔ φ ∈ Logic.Grz := by
+lemma iff_provable_Grz_provable_boxdot_S : Logic.S ⊢! φᵇ ↔ Logic.Grz ⊢! φ := by
   apply Iff.trans iff_provable_boxdot_GL_provable_boxdot_S.symm;
   exact iff_provable_boxdot_GL_provable_Grz;
-
-instance : BoxdotProperty Logic.S Logic.Grz := ⟨iff_provable_Grz_provable_boxdot_S⟩
 
 end LO.Modal.Logic
