Foundation/Modal/Logic/S/Consistent.lean
@@ -9,26 +9,19 @@ open ProvabilityLogic
 open Entailment
 open Kripke Formula.Kripke
 
-lemma iff_provable_GL_provable_box_S {A : Modal.Formula _} : A ∈ Logic.GL ↔ □A ∈ Logic.S := by
+lemma iff_provable_GL_provable_box_S {A : Modal.Formula _} : Logic.GL ⊢! A ↔ Logic.S ⊢! □A := by
   constructor;
   . intro h;
-    apply Logic.sumQuasiNormal.mem₁;
+    apply Logic.sumQuasiNormal.mem₁!;
     apply nec! h;
   . intro h;
     apply GL.arithmetical_completeness (T := 𝐈𝚺₁);
     intro f;
     exact Iff.mp ((𝐈𝚺₁).standardDP 𝐈𝚺₁).sound (S.arithmetical_soundness h f)
 
-theorem S.no_boxbot : □⊥ ∉ Logic.S := by
-  apply iff_provable_GL_provable_box_S.not.mp;
-  apply Logic.no_bot;
+theorem S.no_boxbot : Logic.S ⊬ □⊥ := iff_provable_GL_provable_box_S.not.mp $ by simp;
 
-instance : Logic.S.Consistent := ⟨by
-  apply Set.eq_univ_iff_forall.not.mpr;
-  push_neg;
-  use □⊥;
-  exact Logic.S.no_boxbot;
-⟩
+instance : Entailment.Consistent Logic.S := Entailment.Consistent.of_unprovable S.no_boxbot
 
 end Modal.Logic
 
